---
title: "2-3 Correctness of Horner's rule"
menuTitle: "Problem 2-3"
---

> The following code fragment implements Horner's rule for evaluating a polynomial
>
> <div>
> $$
> \begin{aligned}
> P(x) & = \sum_{k = 0}^n a_k x^k \\
>      & = a_0 + x(a_1 + x (a_2 + \cdots + x(a_{n - 1} + x a_n) \cdots)),
> \end{aligned}
> $$
> </div>
>
> given the coefficients $a\_0, a\_1, \ldots, a\_n$ and a value of $x$:
>
```cpp
    y = 0
        for i = n down 0
        y = ai + x * y
```
>
> **a.** In terms of $\Theta$-notation, what is the running time of this code fragment for Horner's rule?
>
> **b.** Write pseudocode to implement the naive polynomial-evaluation algorithm that computes each term of the polynomial from scratch. What is the running time of this algorithm? How does it compare to Horner's rule 
>
> **c.** Consider the following loop invariant: At the start of each iteration of the **for** loop of lines 2-3, 
>
> <div>
$$
> y = \sum_{k = 0}^{n - (i + 1)} a_{k + i + 1} x^k.
> $$
</div>
>
> Interpret a summation with no terms as equaling $0$. Following the structure of the loop invariant proof presented in this chapter, use this loop invariant to show that, at termination, $y = \sum\_{k = 0}^n a\_k x^k$. 
>
> **d.** Conclude by arguing that the given code fragment correctly evaluates a polynomial characterized by the coefficients $a\_0, a\_1, \ldots, a\_n$.

**a.** $\Theta(n)$.

**b.** 

```cpp
NAIVE-HORNER()
    y = 0
    for k = 0 to n
        temp = 1
        for i = 1 to k
            temp = temp * x
            y = y + ai * m
```

The running time is $\Theta(n^2)$, because of the nested loop. It is obviously slower.

**c.**  **Initialization:** It is pretty trivial, since the summation has no terms which implies $y = 0$.

**Maintenance:** By using the loop invariant, in the end of the $i$-the iteration, we have

<div>
$$
\begin{aligned}
y & = a_i + x \sum_{k = 0}^{n - (i + 1)} a_{k + i + 1} x^k \\
  & = a_i x^0 + \sum_{k = 0}^{n - i - 1} a_{k + i + 1} x^{k + 1} \\
  & = a_i x^0 \sum_{k = 1}^{n - i} a_{k + i} x^k \\
  & = \sum_{k = 0}^{n - i} a_{k + i} x^k.
\end{aligned}
$$
</div>

**Termination:** The loop terminates at $i = -1$. If we substitute,
 
<div>
$$
y = \sum_{k = 0}^{n - i - 1} a_{k + i + 1} x^k = \sum_{k = 0}^n a_k x^k.
$$
</div>

**d.**  The invariant of the loop is a sum that equals a polynomial with the given coefficients.
